Deduction.thy
@@ -1,0 +1,52 @@
+theory Deduction
+  imports Term
+begin
+
+inductive deduce :: "msg set \<Rightarrow> msg \<Rightarrow> bool" ( infix "\<turnstile>" 72)
+  where
+(*do we need T \<turnstile> \<iota> as a rule? *)
+Ax: "u \<in> T \<Longrightarrow> T \<turnstile> u"
+| CompHash: "T \<turnstile> t \<Longrightarrow> T \<turnstile> msg.Hash t"
+| CompPair: "\<lbrakk>T \<turnstile> t1; T \<turnstile> t2\<rbrakk>  \<Longrightarrow> T \<turnstile> msg.Pair t1 t2"
+| CompSenc: "\<lbrakk>T \<turnstile> t1; T \<turnstile> t2\<rbrakk>  \<Longrightarrow> T \<turnstile> msg.Senc t1 t2"
+| CompAenc: "\<lbrakk>T \<turnstile> t1; T \<turnstile> t2\<rbrakk>  \<Longrightarrow> T \<turnstile> msg.Aenc t1 t2"
+| CompSign: "\<lbrakk>T \<turnstile> t\<rbrakk>  \<Longrightarrow> T \<turnstile> msg.Sign t msg.\<iota>"
+| Proj1: "T \<turnstile> msg.Pair t1 t2 \<Longrightarrow> T \<turnstile> t1"
+| Proj2: "T \<turnstile> msg.Pair t1 t2 \<Longrightarrow> T \<turnstile> t2"
+| Sdec: "\<lbrakk>T \<turnstile> msg.Senc t k; T \<turnstile> k\<rbrakk> \<Longrightarrow> T \<turnstile> t"
+| Adec: "\<lbrakk>T \<turnstile> msg.Aenc t msg.\<iota>\<rbrakk> \<Longrightarrow> T \<turnstile> t"
+
+lemma "{msg.Senc (msg.Const ''a'') (msg.Const ''x''), msg.Const ''x''} \<turnstile> (msg.Const ''a'')"
+  apply(rule Sdec)
+   apply(rule Ax)
+   apply auto
+  apply(rule Ax)
+  by auto
+
+lemma "{\<langle>m, n\<rangle>} \<turnstile> \<h>(\<langle>n, m\<rangle>)"
+proof -
+  have 1:"{\<langle>m, n\<rangle>} \<turnstile> (\<langle>m,n\<rangle>)" by (auto intro: Ax)
+  then have 2:"{\<langle>m, n\<rangle>} \<turnstile> m" by (auto intro: Proj1)
+  from 1 have 3:"{\<langle>m, n\<rangle>} \<turnstile> n" by (auto intro:Proj2)
+  from 3 2 have "{\<langle>m, n\<rangle>} \<turnstile> (\<langle>n,m\<rangle>)" by (auto intro:CompPair)
+  thus "{\<langle>m, n\<rangle>} \<turnstile> \<h>(\<langle>n, m\<rangle>)" by (auto intro:CompHash)
+qed
+
+lemma "{\<lbrace>m\<rbrace>\<^sub>k, {k}\<^sub>\<iota>} \<turnstile> (\<langle>m,([k]\<^sub>\<iota>)\<rangle>)" 
+  oops
+
+lemma deduce_weaken:
+assumes "G \<turnstile> t " and "G \<subseteq> H "
+shows "H \<turnstile> t "
+  sorry
+(*proof -
+  obtain x where "x \<in> G" sorry
+  with 2 have "x \<in> H" by auto
+*)
+
+lemma deduce_cut:
+assumes "insert t H \<turnstile> u " and "H \<turnstile> t "
+shows "H \<turnstile> u "
+  sorry
+
+end
